Weakening/monotonicity

PdlParallelStoring/AxiomaticSystem.lean
@@ -2,7 +2,7 @@ import Mathlib.Data.Set.Basic
 
 import PdlParallelStoring.Syntax
 
--- TODO: Call this module DeductiveSystem (?)
+open Program
 
 ----------------------------------------------------------------------------------------------------
 -- Axiomatic System for RSPDL₀ (Hilbert-style with context)
@@ -10,34 +10,45 @@ import PdlParallelStoring.Syntax
 -- This is a fragment called RSPDL₀. In this fragment, we do not allow the use of the operators of
 -- test (?), iteration (★) and parallel composition (‖).
 
-inductive Axiom : Φ → Prop where
+inductive Axiom : Formula → Prop where
+  -- Classical Logic Axioms
+  | contradiction φ : Axiom ((φ ∧ (¬ φ)) → ⊥')
+  | reductio φ : Axiom (((¬ φ) → ⊥') → φ)
+  | conjIntro φ ψ : Axiom (φ → (ψ → (φ ∧ ψ)))
+  | conjElimL φ ψ : Axiom ((φ ∧ ψ) → φ)
+  | conjElimR φ ψ : Axiom ((φ ∧ ψ) → ψ)
   -- Modal Axioms
   | composition α β φ : Axiom (([α ; β] φ) ↔ ([α] [β] φ))
   | choice α β φ : Axiom (([α ∪ β] φ) ↔ (([α] φ) ∧ ([β] φ)))
   | K α φ₁ φ₂ : Axiom (([α] (φ₁ → φ₂)) → (([α] φ₁) → ([α] φ₂)))
   -- RSPDL₀ Specific Axioms
-  | functionalR₁ φ : Axiom ((⟨π.r₁⟩ φ) → ([π.r₁] φ))
-  | functionalR₂ φ : Axiom ((⟨π.r₂⟩ φ) → ([π.r₂] φ))
-  | temporalForward φ : Axiom (φ → ([π.s₁] ⟨π.r₁⟩ φ))
-  | temporalBackward φ : Axiom (⟨π.s₁⟩ ⟨π.r₁⟩ φ → φ)
-  | s₁r₁Converse φ : Axiom ((⟨π.s₁⟩ φ) → (⟨π.r₁⟩ φ))
-  | r₁s₁Converse φ : Axiom ((⟨π.r₁⟩ φ) → (⟨π.s₁⟩ φ))
-  | temporalForward₂ φ : Axiom (φ → ([π.s₂] ⟨π.r₂⟩ φ))
-  | temporalBackward₂ φ : Axiom (⟨π.s₂⟩ ⟨π.r₂⟩ φ → φ)
-  | s₂r₂Converse φ : Axiom ((⟨π.s₂⟩ φ) → (⟨π.r₂⟩ φ))
-  | r₂s₂Converse φ : Axiom (⟨π.r₂⟩ φ → (⟨π.s₂⟩ φ))
-  | sameDomain : Axiom ((⟨π.r₁⟩ ⊤') ↔ (⟨π.r₂⟩ ⊤'))
-  | unicity φ : Axiom ((⟨π.s₁ ; π.r₁⟩ φ) ↔ ([π.s₁ ; π.r₁] φ))
-  | storeRestoreId φ : Axiom (([π.s₁ ; π.r₂] φ) → φ)
-  | storeRestoreDiamond φ : Axiom (φ → ([π.s₁ ; π.r₂] ⟨π.s₁ ; π.r₂⟩ φ))
-  | storeRestoreIterate φ : Axiom (([π.s₁ ; π.r₂] φ) → ([π.s₁ ; π.r₂] [π.s₁ ; π.r₂] φ))
+  | functionalR₁ φ : Axiom ((⟨r₁⟩ φ) → ([r₁] φ))
+  | functionalR₂ φ : Axiom ((⟨r₂⟩ φ) → ([r₂] φ))
+  | temporalForward φ : Axiom (φ → ([s₁] ⟨r₁⟩ φ))
+  | temporalBackward φ : Axiom (⟨s₁⟩ ⟨r₁⟩ φ → φ)
+  | s₁r₁Converse φ : Axiom ((⟨s₁⟩ φ) → (⟨r₁⟩ φ))
+  | r₁s₁Converse φ : Axiom ((⟨r₁⟩ φ) → (⟨s₁⟩ φ))
+  | temporalForward₂ φ : Axiom (φ → ([s₂] ⟨r₂⟩ φ))
+  | temporalBackward₂ φ : Axiom (⟨s₂⟩ ⟨r₂⟩ φ → φ)
+  | s₂r₂Converse φ : Axiom ((⟨s₂⟩ φ) → (⟨r₂⟩ φ))
+  | r₂s₂Converse φ : Axiom (⟨r₂⟩ φ → (⟨s₂⟩ φ))
+  | sameDomain : Axiom ((⟨r₁⟩ ⊤') ↔ (⟨r₂⟩ ⊤'))
+  | unicity φ : Axiom ((⟨s₁ ; r₁⟩ φ) ↔ ([s₁ ; r₁] φ))
+  | storeRestoreId φ : Axiom (([s₁ ; r₂] φ) → φ)
+  | storeRestoreDiamond φ : Axiom (φ → ([s₁ ; r₂] ⟨s₁ ; r₂⟩ φ))
+  | storeRestoreIterate φ : Axiom (([s₁ ; r₂] φ) → ([s₁ ; r₂] [s₁ ; r₂] φ))
 
 -- Deduction system with context.
-inductive Deduction : Set Φ → Φ → Prop where
-  | premise (Γ : Set Φ) (φ : Φ) : (φ ∈ Γ) → Deduction Γ φ
-  | axiom' (Γ : Set Φ) (φ : Φ) : Axiom φ → Deduction Γ φ
-  | modusPonens (Γ : Set Φ) (φ ψ : Φ) : Deduction Γ φ → Deduction Γ (φ → ψ) → Deduction Γ ψ
-  | necessitation (Γ : Set Φ) (α : π) (φ : Φ) : Deduction ∅ φ → Deduction Γ ([α] φ)
+inductive Deduction : Set Formula → Formula → Prop where
+  | premise (Γ : Set Formula) (φ : Formula) : (φ ∈ Γ) → Deduction Γ φ
+  | axiom' (Γ : Set Formula) (φ : Formula) : Axiom φ → Deduction Γ φ
+  | modusPonens (Γ : Set Formula) (φ ψ : Formula) :
+      Deduction Γ φ →
+      Deduction Γ (φ → ψ) →
+      Deduction Γ ψ
+  | necessitation (Γ : Set Formula) (α : Program) (φ : Formula) :
+      Deduction ∅ φ →
+      Deduction Γ ([α] φ)
 
 notation:40 Γ " ⊢ " φ => Deduction Γ φ
 
