PdlParallelStoring/Completeness.lean
@@ -11,50 +11,117 @@ open Classical
 --   - iteration (★)
 --   - parallel composition (‖).
 
-def IsConsistent (Γ : Set Φ) : Prop :=
+def IsConsistent (Γ : Set Formula) : Prop :=
   ¬ (Γ ⊢ ⊥')
 
-def IsMaximalConsistent (Γ : Set Φ) : Prop :=
+def IsMaximalConsistent (Γ : Set Formula) : Prop :=
   IsConsistent Γ ∧
   ∀ {φ}, (φ ∉ Γ) → ¬ IsConsistent (Γ ∪ {φ})
 
 lemma consistent_empty : IsConsistent ∅ := by
   sorry
 
-lemma deduction_consistency (φ : Φ) : ((⊢ φ) ↔ ¬ IsConsistent {¬ φ}) := by
+lemma weakening : ∀ {Γ Δ : Set Formula} {φ : Formula}, (Γ ⊆ Δ) → (Γ ⊢ φ) → Δ ⊢ φ := by
+  intros _ _ _ h_sub h_deriv
+  induction h_deriv with
+  | premise _ _ h_mem =>
+      apply Deduction.premise
+      exact h_sub h_mem
+  | axiom' _ _ h_ax =>
+      apply Deduction.axiom'
+      exact h_ax
+  | modusPonens _ _ _ _ _ ih_phi ih_imp =>
+      apply Deduction.modusPonens
+      · exact ih_phi h_sub
+      · exact ih_imp h_sub
+  | necessitation _ _ _ h_empty _ =>
+      apply Deduction.necessitation
+      exact h_empty
+
+lemma monotonicity : ∀ {Γ Δ : Set Formula} {φ : Formula}, (Γ ⊢ φ) → (Γ ∪ Δ) ⊢ φ := by
+  intros _ _ _ h_deriv
+  apply weakening
+  · intro _ hx
+    left
+    exact hx
+  · exact h_deriv
+
+lemma deduction_theorem : ∀ {Γ : Set Formula} {φ ψ : Formula},
+    (Γ ∪ {φ} ⊢ ψ) → (Γ ⊢ (φ → ψ)) := by
+  intros Γ φ ψ h_union_deriv
   sorry
 
-lemma unprovable_consistent (φ : Φ) : (¬ ⊢ φ) → IsConsistent {¬ φ} := by
-  intros hNotProv
-  rewrite [deduction_consistency φ] at hNotProv
-  exact Decidable.not_not.mp hNotProv
+lemma deduction_consistency_aux : ∀ {Γ : Set Formula} {φ : Formula},
+    (Γ ⊢ φ) ↔ ¬ IsConsistent (Γ ∪ {¬ φ}) := by
+  intros Γ φ
+  constructor
+  . intros h_deriv h_consist
+    apply h_consist
+    have h₁ : Γ ∪ {¬ φ} ⊢ φ := monotonicity h_deriv
+    have h₂ : Γ ∪ {¬ φ} ⊢ ¬ φ := by
+      apply Deduction.premise
+      simp only [Set.union_singleton, Set.mem_insert_iff, true_or]
+    have h₃ : Γ ∪ {¬ φ} ⊢ φ ∧ ¬ φ := by
+      have h_ax : (Γ ∪ {¬ φ}) ⊢ (φ → ((¬ φ) → (φ ∧ (¬ φ)))) := by
+        apply Deduction.axiom'
+        apply Axiom.conjIntro
+      have h_step : (Γ ∪ {¬ φ}) ⊢ ((¬ φ) → (φ ∧ (¬ φ))) := by
+        exact Deduction.modusPonens (Γ ∪ {¬ φ}) φ ((¬ φ) → (φ ∧ (¬ φ))) h₁ h_ax
+      exact Deduction.modusPonens (Γ ∪ {¬ φ}) (¬ φ) (φ ∧ (¬ φ)) h₂ h_step
+    have h₄ : Γ ∪ {¬ φ} ⊢ ((φ ∧ (¬ φ)) → ⊥') := by
+      apply Deduction.axiom'
+      apply Axiom.contradiction
+    exact Deduction.modusPonens (Γ ∪ {¬ φ}) (φ ∧ (¬ φ)) ⊥' h₃ h₄
+  . intros h_inconsistent
+    simp only [IsConsistent, Decidable.not_not] at h_inconsistent
+    have h_imp : Γ ⊢ ((¬ φ) → ⊥') := deduction_theorem h_inconsistent
+    apply Deduction.modusPonens Γ ((¬ φ) → ⊥') φ h_imp
+    apply Deduction.axiom'
+    apply Axiom.reductio
+
+lemma deduction_consistency : ∀ {φ : Formula}, ((⊢ φ) ↔ ¬ IsConsistent {¬ φ}) := by
+  intros φ
+  constructor
+  . sorry
+  . sorry
+
+lemma unprovable_consistent : ∀ {φ : Formula}, (¬ ⊢ φ) → IsConsistent {¬ φ} := by
+  intros _ h_not_prov
+  rewrite [deduction_consistency] at h_not_prov
+  exact Decidable.not_not.mp h_not_prov
 
 def MaximalConsistentSet : Type :=
-  {Γ : Set Φ // IsMaximalConsistent Γ}
+  {Γ : Set Formula // IsMaximalConsistent Γ}
 
-lemma mcs_complete (Γ : MaximalConsistentSet) (φ : Φ) : (φ ∈ Γ.val) ∨ (¬ φ) ∈ Γ.val := by
+lemma mcs_complete (Γ : MaximalConsistentSet) (φ : Formula) : (φ ∈ Γ.val) ∨ (¬ φ) ∈ Γ.val := by
   sorry
 
-lemma mcs_no_contradiction (Γ : MaximalConsistentSet) (φ : Φ) : (φ ∈ Γ.val) → (¬ φ) ∉ Γ.val := by
+lemma mcs_no_contradiction (Γ : MaximalConsistentSet) (φ : Formula) :
+    (φ ∈ Γ.val) →
+    (¬ φ) ∉ Γ.val := by
   sorry
 
 namespace Lindenbaum
 
-def insert : Option Φ → Set Φ → Set Φ
+def insert : Option Formula → Set Formula → Set Formula
   | none, Γ => Γ
   | some φ, Γ =>
       if IsConsistent (Γ ∪ {φ})
       then Γ ∪ {φ}
       else Γ ∪ {¬ φ}
 
-def delta (Γ : Set Φ) : Nat → Set Φ
+def delta (Γ : Set Formula) : Nat → Set Formula
   | 0 => Γ
   | n + 1 => insert (decode n) (delta Γ n)
 
-def max (Γ : Set Φ) : Set Φ :=
+def max (Γ : Set Formula) : Set Formula :=
   ⋃ n, delta Γ n
 
-lemma cut_aux : ∀ {Δ ψ}, (Δ ⊢ ψ) → ∀ {Γ φ}, (Δ = (Γ ∪ {φ})) → (Γ ⊢ φ) → Γ ⊢ ψ := by
+lemma cut_aux :
+    ∀ {Δ : Set Formula} {ψ : Formula}, (Δ ⊢ ψ) →
+    ∀ {Γ: Set Formula} {φ: Formula}, (Δ = (Γ ∪ {φ})) →
+    (Γ ⊢ φ) →
+    Γ ⊢ ψ := by
   intros _ _ h
   induction h with
   | premise _ φ h_in =>
@@ -69,52 +136,72 @@ lemma cut_aux : ∀ {Δ ψ}, (Δ ⊢ ψ) → ∀ {Γ φ}, (Δ = (Γ ∪ {φ})) �
   | axiom' _ φ h_ax =>
       intros Δ _ _ _
       exact Deduction.axiom' Δ φ h_ax
-  | modusPonens Γ φ ψ h_ant h_cond ih₁ ih₂ =>
-      intros Δ χ h_eq h_deriv
-      sorry
-  | necessitation =>
-      sorry
+  | modusPonens _ φ ψ _ _ ih₁ ih₂ =>
+      intros Δ _ h_eq h_deriv
+      have h_ant : Δ ⊢ φ := ih₁ h_eq h_deriv
+      have h_cond : Δ ⊢ (φ → ψ) := ih₂ h_eq h_deriv
+      exact Deduction.modusPonens Δ φ ψ h_ant h_cond
+  | necessitation _ α φ h_empty_deriv _ =>
+      intros Δ _ _ _
+      exact Deduction.necessitation Δ α φ h_empty_deriv
 
-theorem cut : ∀ {φ ψ : Φ}, (Γ ⊢ φ) → (Γ ∪ {φ} ⊢ ψ) → Γ ⊢ ψ := by
-  intros φ ψ h₁ h₂
+lemma cut : ∀ {Γ : Set Formula} {φ ψ : Formula}, (Γ ⊢ φ) → (Γ ∪ {φ} ⊢ ψ) → Γ ⊢ ψ := by
+  intros _ _ _ h₁ h₂
   exact cut_aux h₂ rfl h₁
 
-lemma consistency_either (Γ : Set Φ) (φ : Φ) :
+lemma consistency_either (Γ : Set Formula) (φ : Formula) :
     IsConsistent Γ →
     IsConsistent (Γ ∪ {φ}) ∨ IsConsistent (Γ ∪ {¬ φ}) := by
-  sorry
+  intros h_consistent
+  by_contra h
+  have h₁ : (¬ IsConsistent (Γ ∪ {φ})) ∧ ¬ IsConsistent (Γ ∪ {¬ φ}) := by
+    constructor
+    . intros h_union_consistent
+      apply h
+      left
+      exact h_union_consistent
+    . intros h_union_consistent
+      apply h
+      right
+      exact h_union_consistent
+  obtain ⟨h₁₁, h₁₂⟩ := h₁
+  rewrite [← deduction_consistency_aux] at h₁₂
+  apply h₁₁
+  intros h₂
+  apply h_consistent
+  exact cut h₁₂ h₂
 
-lemma insert_preserves_consistency (opt_φ : Option Φ) (Γ : Set Φ) :
-    IsConsistent Γ → IsConsistent (insert opt_φ Γ) := by
-  intros hConsistent
+lemma insert_preserves_consistency (opt_φ : Option Formula) (Γ : Set Formula) :
+    IsConsistent Γ →
+    IsConsistent (insert opt_φ Γ) := by
+  intros h_consistent
   cases opt_φ with
-  | none => exact hConsistent
+  | none => exact h_consistent
   | some φ =>
       rewrite [insert]
       split_ifs with h
       . exact h
-      . have hEither := consistency_either Γ φ hConsistent
-        cases hEither with
+      . have h_either := consistency_either Γ φ h_consistent
+        cases h_either with
         | inl _ => contradiction
         | inr hRight => exact hRight
 
-lemma delta_preserves_consistency (Γ : Set Φ) (n : Nat) :
-    IsConsistent Γ → IsConsistent (delta Γ n) := by
-  intros hConsistent
+lemma delta_preserves_consistency (Γ : Set Formula) (n : Nat) :
+    IsConsistent Γ →
+    IsConsistent (delta Γ n) := by
+  intros h_consistent
   induction n with
-  | zero => exact hConsistent
+  | zero => exact h_consistent
   | succ n ih =>
       apply insert_preserves_consistency
       exact ih
 
-lemma lindenbaum (Γ : Set Φ) : IsConsistent Γ → ∃ (Δ : MaximalConsistentSet), Γ ⊆ Δ.val := by
-  /- intros hConsistent -/
-  /- exists (max Γ) -/
+lemma lindenbaum (Γ : Set Formula) : IsConsistent Γ → ∃ (Δ : MaximalConsistentSet), Γ ⊆ Δ.val := by
   sorry
 
 end Lindenbaum
 
-def canonicalRelation (α : π) (Γ Δ : MaximalConsistentSet) : Prop :=
+def canonicalRelation (α : Program) (Γ Δ : MaximalConsistentSet) : Prop :=
   ∀ {φ}, (([α] φ) ∈ Γ.val) → φ ∈ Δ.val
 
 def canonicalFrame : Frame where
@@ -123,13 +210,14 @@ def canonicalFrame : Frame where
   nonempty := sorry
 
 def canonicalValuation (lit : Literal) (Γ : MaximalConsistentSet) : Prop :=
-  (Φ.atomic lit) ∈ Γ.val
+  (Formula.atomic lit) ∈ Γ.val
 
 def canonicalModel : Model where
   F := canonicalFrame
   V := canonicalValuation
 
-lemma truth_lemma (φ : Φ) (Γ : canonicalModel.F.W) : ((canonicalModel, Γ) ⊨ φ) ↔ φ ∈ Γ.val := by
+lemma truth_lemma (φ : Formula) (Γ : canonicalModel.F.W) :
+    ((canonicalModel, Γ) ⊨ φ) ↔ φ ∈ Γ.val := by
   sorry
 
 instance canonicalProper : Proper canonicalFrame := by
@@ -143,27 +231,27 @@ instance : ProperStandard canonicalModel where
   toProper := canonicalProper
 
 lemma contrapositive_completeness :
-    ∀ {φ : Φ}, (¬ ⊢ φ) →
+    ∀ {φ : Formula}, (¬ ⊢ φ) →
     ∃ (M : Model) (_ : ProperStandard M), ¬ (M ⊨ φ) := by
-  intros φ hNotProv
-  have h₁ : IsConsistent {¬ φ} := unprovable_consistent φ hNotProv
+  intros φ h_not_prov
+  have h₁ : IsConsistent {¬ φ} := unprovable_consistent h_not_prov
   obtain ⟨Γ, h₂⟩ := Lindenbaum.lindenbaum {¬ φ} h₁
   have h₃ : (¬ φ) ∈ Γ.val := h₂ (Set.mem_singleton (¬ φ))
   have h₄ : φ ∉ Γ.val := by
-    by_contra hIn
-    have hNotIn : (¬ φ) ∉ Γ.val := mcs_no_contradiction Γ φ hIn
-    exact hNotIn h₃
+    by_contra h_in
+    have h_not_in : (¬ φ) ∉ Γ.val := mcs_no_contradiction Γ φ h_in
+    exact h_not_in h₃
   have h₅ : ¬ ((canonicalModel, Γ) ⊨ φ) := by
     rewrite [truth_lemma φ Γ]
     exact h₄
   use canonicalModel, inferInstance
-  intro hGlobalSat
-  have hSat : (canonicalModel, Γ) ⊨ φ := hGlobalSat
-  exact h₅ hSat
+  intro h_global_sat
+  have h_sat : (canonicalModel, Γ) ⊨ φ := h_global_sat
+  exact h₅ h_sat
 
-theorem completeness : ∀ {φ : Φ}, (⊨ φ) → (⊢ φ) := by
-  intros φ hValid
-  by_contra hNotProv
-  obtain ⟨M, _, hNotGlobalSat⟩ := contrapositive_completeness hNotProv
-  have hGlobalSat : M ⊨ φ := hValid rfl
-  exact hNotGlobalSat hGlobalSat
+theorem completeness : ∀ {φ : Formula}, (⊨ φ) → (⊢ φ) := by
+  intros φ h_valid
+  by_contra h_not_prov
+  obtain ⟨M, _, h_not_global_sat⟩ := contrapositive_completeness h_not_prov
+  have h_global_sat : M ⊨ φ := h_valid rfl
+  exact h_not_global_sat h_global_sat
