PdlParallelStoring/Properties.lean
@@ -1,24 +1,25 @@
 import PdlParallelStoring.Semantics
 
+open Program
+
 ----------------------------------------------------------------------------------------------------
 -- Properties of Proper Structured Frames
 ----------------------------------------------------------------------------------------------------
 -- Property I) Rs₁ ; Rr₁ = Id
 @[simp]
-lemma s₁_comp_r₁ (F : Frame) [P : Proper F] :
-    ∀ {s u}, Relation.Comp (F.R π.s₁) (F.R π.r₁) s u ↔
-             s = u := by
+lemma s₁_comp_r₁ (F : Frame) [P : Proper F] : ∀ {s u : F.W},
+    Relation.Comp (F.R s₁) (F.R r₁) s u ↔ s = u := by
   intros s u
   constructor
   . intro hcomp
     obtain ⟨t, hs₁, hr₁⟩ := hcomp
-    rw [P.s₁] at hs₁
-    rw [P.r₁] at hr₁
+    rewrite [P.s₁] at hs₁
+    rewrite [P.r₁] at hr₁
     obtain ⟨s₁, t₁, hs_eq, ht_eq⟩ := hs₁
     obtain ⟨s₂, t₂, ht_eq₂, hu_eq⟩ := hr₁
     have h_eq : s₁ ⋆ t₁ = s₂ ⋆ t₂ := by rw [← ht_eq, ht_eq₂]
     have s₁_eq_s₂ : s₁ = s₂ := (State.inject.mp h_eq).1
-    rw [hs_eq, hu_eq]
+    rewrite [hs_eq, hu_eq]
     exact s₁_eq_s₂
   . intro h_eq
     use s ⋆ s
@@ -28,20 +29,19 @@ lemma s₁_comp_r₁ (F : Frame) [P : Proper F] :
 
 -- Property II) Rs₂ ; Rr₂ = Id
 @[simp]
-lemma s₂_comp_r₂ (F : Frame) [P : Proper F] :
-    ∀ {s u}, Relation.Comp (F.R π.s₂) (F.R π.r₂) s u ↔
-             s = u := by
+lemma s₂_comp_r₂ (F : Frame) [P : Proper F] : ∀ {s u : F.W},
+    Relation.Comp (F.R s₂) (F.R r₂) s u ↔ s = u := by
   intros s u
   constructor
   . intro hcomp
     obtain ⟨t, hs₂, hr₂⟩ := hcomp
-    rw [P.s₂] at hs₂
-    rw [P.r₂] at hr₂
+    rewrite [P.s₂] at hs₂
+    rewrite [P.r₂] at hr₂
     obtain ⟨s₁, t₁, hs_eq, ht_eq⟩ := hs₂
     obtain ⟨s₂, t₂, ht_eq₂, hu_eq⟩ := hr₂
     have h_eq : s₁ ⋆ t₁ = s₂ ⋆ t₂ := by rw [← ht_eq, ht_eq₂]
     have t₁_eq_t₂ : t₁ = t₂ := (State.inject.mp h_eq).2
-    rw [hs_eq, hu_eq]
+    rewrite [hs_eq, hu_eq]
     exact t₁_eq_t₂
   . intro h_eq
     use s ⋆ s
@@ -50,47 +50,45 @@ lemma s₂_comp_r₂ (F : Frame) [P : Proper F] :
 
 -- Property III) Rs₁ ; Rr₂ = E
 @[simp]
-lemma s₁_comp_r₂ (F : Frame) [P : Proper F] :
-    ∀ {s t}, Relation.Comp (F.R π.s₁) (F.R π.r₂) s t ↔
-             s ≈ t := by
+lemma s₁_comp_r₂ (F : Frame) [P : Proper F] : ∀ {s t : F.W},
+    Relation.Comp (F.R s₁) (F.R r₂) s t ↔ s ≈ t := by
   intros s t
   constructor
   . intro hcomp
     obtain ⟨_, hs₁, hr₂⟩ := hcomp
-    rw [P.s₁, P.r₂] at *
+    rewrite [P.s₁, P.r₂] at *
     obtain ⟨s₁, t₁, hs_eq, hu_eq⟩ := hs₁
     obtain ⟨s₂, t₂, hu_eq₂, ht_eq⟩ := hr₂
     have h_eq : s₁ ⋆ t₁ = s₂ ⋆ t₂ := by rw [← hu_eq, hu_eq₂]
     have ⟨_, t₁_eq_t₂⟩ := State.inject.mp h_eq
-    rw [hs_eq, ht_eq, ← t₁_eq_t₂]
+    rewrite [hs_eq, ht_eq, ← t₁_eq_t₂]
     have h₁ : s₁ ≈ (s₁ ⋆ t₁) := by
       apply Structured.respects_equiv
-      rw [P.s₁]
+      rewrite [P.s₁]
       use s₁, t₁
     have h₂ : t₁ ≈ (s₁ ⋆ t₁) := by
       apply Structured.respects_equiv
-      rw [P.s₂]
+      rewrite [P.s₂]
       use s₁, t₁
     have h₃ : (s₁ ⋆ t₁) ≈ t₁ := State.equiv.symm h₂
     exact State.equiv.trans h₁ h₃
   . intro _
     use s ⋆ t
-    rw [P.s₁, P.r₂] at *
+    rewrite [P.s₁, P.r₂] at *
     constructor
     . use s, t
     . use s, t
 
 -- Property IV) (Rr₁ ; Rs₁) ∩ (Rr₂ ; Rs₂) ⊆ Id
 @[simp]
-lemma r₁_s₁_inter_r₂_s₂ (F : Frame) [P : Proper F] :
-    ∀ {s t}, (Relation.Comp (F.R π.r₁) (F.R π.s₁) s t ∧
-              Relation.Comp (F.R π.r₂) (F.R π.s₂) s t) →
-              s = t := by
+lemma r₁_s₁_inter_r₂_s₂ (F : Frame) [P : Proper F] : ∀ {s t : F.W},
+    (Relation.Comp (F.R r₁) (F.R s₁) s t ∧ Relation.Comp (F.R r₂) (F.R s₂) s t) →
+    s = t := by
   intros s t hcomp
   obtain ⟨hcomp₁, hcomp₂⟩ := hcomp
   obtain ⟨i₁, hr₁, hs₁⟩ := hcomp₁
   obtain ⟨i₂, hr₂, hs₂⟩ := hcomp₂
-  rw [P.s₁, P.s₂, P.r₁, P.r₂] at *
+  rewrite [P.s₁, P.s₂, P.r₁, P.r₂] at *
   obtain ⟨s₁, t₁, hs_eq₁, hi₁_eq₁⟩ := hr₁
   obtain ⟨s₂, t₂, hi₁_eq₂, ht_eq₁⟩ := hs₁
   obtain ⟨s₃, t₃, hs_eq₂, hi₂_eq₁⟩ := hr₂
@@ -98,11 +96,11 @@ lemma r₁_s₁_inter_r₂_s₂ (F : Frame) [P : Proper F] :
   conv at ht_eq₂ =>
     rhs
     arg 2
-    rw [← hi₂_eq₂, hi₂_eq₁]
+    rewrite [← hi₂_eq₂, hi₂_eq₁]
   conv at ht_eq₁ =>
     rhs
     arg 1
-    rw [← hi₁_eq₂, hi₁_eq₁]
+    rewrite [← hi₁_eq₂, hi₁_eq₁]
   have h₁ : s₁ ⋆ t₁ = s₃ ⋆ t₃ := by rw [← hs_eq₁, hs_eq₂]
   have ⟨_, t₁_eq_t₃⟩ := State.inject.mp h₁
   have h₂ : s₁ ⋆ t₂ = s₄ ⋆ t₃ := by rw [← ht_eq₁, ht_eq₂]
@@ -112,38 +110,37 @@ lemma r₁_s₁_inter_r₂_s₂ (F : Frame) [P : Proper F] :
 
 -- Property V) Rr₁ ; E = Rr₂ ; E
 @[simp]
-lemma r₁_E_eq_r₂_E (F : Frame) [P : Proper F] :
-    ∀ {s t}, Relation.Comp (F.R π.r₁) State.E s t ↔
-             Relation.Comp (F.R π.r₂) State.E s t := by
+lemma r₁_E_eq_r₂_E (F : Frame) [P : Proper F] : ∀ {s t : F.W},
+    Relation.Comp (F.R r₁) State.E s t ↔ Relation.Comp (F.R r₂) State.E s t := by
   intros s t
   constructor
   . intros comp
     obtain ⟨i, hr₁, equiv⟩ := comp
-    rw [P.r₁] at hr₁
+    rewrite [P.r₁] at hr₁
     obtain ⟨s₁, t₁, s_eq, i_eq⟩ := hr₁
     use t₁
     constructor
-    . rw [P.r₂, s_eq]
+    . rewrite [P.r₂, s_eq]
       use s₁, t₁
-    . rw [← s₁_comp_r₂]
+    . rewrite [← s₁_comp_r₂]
       use t₁ ⋆ t
       constructor
-      . rw [P.s₁]
+      . rewrite [P.s₁]
         use t₁, t
-      . rw [P.r₂]
+      . rewrite [P.r₂]
         use t₁, t
   . intros comp
     obtain ⟨i, hr₂, equiv⟩ := comp
-    rw [P.r₂] at hr₂
+    rewrite [P.r₂] at hr₂
     obtain ⟨s₁, t₁, s_eq, i_eq⟩ := hr₂
     use s₁
     constructor
-    . rw [s_eq, P.r₁]
+    . rewrite [s_eq, P.r₁]
       use s₁, t₁
-    . rw [← s₁_comp_r₂]
+    . rewrite [← s₁_comp_r₂]
       use s₁ ⋆ t
       constructor
-      . rw [P.s₁]
+      . rewrite [P.s₁]
         use s₁, t
-      . rw [P.r₂]
+      . rewrite [P.r₂]
         use s₁, t
